Lean4Lean/Verify.lean
@@ -6,5 +6,6 @@ SPDX-License-Identifier: Apache-2.0 AND (MIT OR Apache-2.0)
 
 import Lean4Lean.Verify.Typing.Lemmas
 import Lean4Lean.Verify.ConditionReflect
+import Lean4Lean.Verify.ModDivCondition
 import Lean4Lean.Verify.Environment
 import Lean4Lean.Verify.Environment.InductiveReplayMatrix
